src/sequential/SeqLiftStep.v
@@ -38,291 +38,728 @@ Require Import Lia.
 Require Import SeqLift.
 (* Require Import Simple. *)
 
-Section LANG.
-  Variable lang_src: language.
-  Variable lang_tgt: language.
 
-  Record sim_tview
-         (f: Mapping.ts)
-         (flag_src: Loc.t -> option Time.t)
-         (rel_vers: Loc.t -> version)
-         (tvw_src: TView.t) (tvw_tgt: TView.t)
-    :
-      Prop :=
-    sim_tview_intro {
-        sim_tview_rel: forall loc,
-          sim_view (fun loc0 => loc0 <> loc) f (rel_vers loc) (tvw_src.(TView.rel) loc) (tvw_tgt.(TView.rel) loc);
-        sim_tview_cur: sim_view (fun loc => flag_src loc = None) f (Mapping.vers f) tvw_src.(TView.cur) tvw_tgt.(TView.cur);
-        sim_tview_acq: sim_view (fun loc => flag_src loc = None) f (Mapping.vers f) tvw_src.(TView.acq) tvw_tgt.(TView.acq);
-      }.
+Lemma sim_timemap_mon_latest L f0 f1 tm_src tm_tgt
+      (SIM: sim_timemap L f0 (Mapping.vers f0) tm_src tm_tgt)
+      (LE: Mapping.les f0 f1)
+      (WF0: Mapping.wfs f0)
+      (WF1: Mapping.wfs f1)
+  :
+    sim_timemap L f1 (Mapping.vers f1) tm_src tm_tgt.
+Proof.
+  eapply sim_timemap_mon_ver; auto.
+  { erewrite <- sim_timemap_mon_mapping; eauto. eapply mapping_latest_wf. }
+  { eapply version_le_version_wf.
+    eapply version_wf_mapping_mon; eauto. eapply mapping_latest_wf.
+  }
+  { eapply mapping_latest_wf. }
+Qed.
 
-  Lemma sim_tview_tgt_mon f flag_src rel_vers tvw_src tvw_tgt0 tvw_tgt1
-        (SIM: sim_tview f flag_src rel_vers tvw_src tvw_tgt0)
-        (TVIEW: TView.le tvw_tgt0 tvw_tgt1)
-    :
-      sim_tview f flag_src rel_vers tvw_src tvw_tgt1.
-  Proof.
-    econs.
-    { i. eapply sim_view_mon_tgt.
-      { eapply SIM. }
-      { eapply TVIEW. }
+Lemma sim_view_mon_latest L f0 f1 vw_src vw_tgt
+      (SIM: sim_view L f0 (Mapping.vers f0) vw_src vw_tgt)
+      (LE: Mapping.les f0 f1)
+      (WF0: Mapping.wfs f0)
+      (WF1: Mapping.wfs f1)
+  :
+    sim_view L f1 (Mapping.vers f1) vw_src vw_tgt.
+Proof.
+  econs.
+  { eapply sim_timemap_mon_latest; eauto. eapply SIM. }
+  { eapply sim_timemap_mon_latest; eauto. eapply SIM. }
+Qed.
+
+Record sim_tview
+       (f: Mapping.ts)
+       (flag_src: Loc.t -> option Time.t)
+       (rel_vers: Loc.t -> version)
+       (tvw_src: TView.t) (tvw_tgt: TView.t)
+  :
+    Prop :=
+  sim_tview_intro {
+      sim_tview_rel: forall loc,
+        sim_view (fun loc0 => loc0 <> loc) f (rel_vers loc) (tvw_src.(TView.rel) loc) (tvw_tgt.(TView.rel) loc);
+      sim_tview_cur: sim_view (fun loc => flag_src loc = None) f (Mapping.vers f) tvw_src.(TView.cur) tvw_tgt.(TView.cur);
+      sim_tview_acq: sim_view (fun loc => flag_src loc = None) f (Mapping.vers f) tvw_src.(TView.acq) tvw_tgt.(TView.acq);
+      rel_vers_wf: forall loc, version_wf f (rel_vers loc);
+    }.
+
+Lemma sim_tview_mon_latest f0 f1 flag_src rel_vers tvw_src tvw_tgt
+      (SIM: sim_tview f0 flag_src rel_vers tvw_src tvw_tgt)
+      (LE: Mapping.les f0 f1)
+      (WF0: Mapping.wfs f0)
+      (WF1: Mapping.wfs f1)
+  :
+    sim_tview f1 flag_src rel_vers tvw_src tvw_tgt.
+Proof.
+  econs.
+  { i. erewrite <- sim_view_mon_mapping; [eapply SIM|..]; eauto. eapply SIM. }
+  { eapply sim_view_mon_latest; eauto. eapply SIM. }
+  { eapply sim_view_mon_latest; eauto. eapply SIM. }
+  { i. eapply version_wf_mapping_mon; eauto. eapply SIM. }
+Qed.
+
+Lemma sim_tview_tgt_mon f flag_src rel_vers tvw_src tvw_tgt0 tvw_tgt1
+      (SIM: sim_tview f flag_src rel_vers tvw_src tvw_tgt0)
+      (TVIEW: TView.le tvw_tgt0 tvw_tgt1)
+  :
+    sim_tview f flag_src rel_vers tvw_src tvw_tgt1.
+Proof.
+  econs.
+  { i. eapply sim_view_mon_tgt.
+    { eapply SIM. }
+    { eapply TVIEW. }
+  }
+  { eapply sim_view_mon_tgt.
+    { eapply SIM. }
+    { eapply TVIEW. }
+  }
+  { eapply sim_view_mon_tgt.
+    { eapply SIM. }
+    { eapply TVIEW. }
+  }
+  { eapply SIM. }
+Qed.
+
+Variant wf_release_vers (vers: versions) (prom_tgt: Memory.t) (rel_vers: Loc.t -> version): Prop :=
+| wf_release_vers_intro
+    (PROM: forall loc from to val released
+                  (GET: Memory.get loc to prom_tgt = Some (from, Message.concrete val (Some released))),
+        exists v,
+          (<<VER: vers loc to = Some v>>) /\
+          (<<REL: rel_vers loc = v>>))
+.
+
+Variant sim_local
+        (f: Mapping.ts) (vers: versions)
+        (flag_src: Loc.t -> option Time.t)
+        (flag_tgt: Loc.t -> option Time.t)
+  :
+    Local.t -> Local.t -> Prop :=
+| sim_local_intro
+    tvw_src tvw_tgt prom_src prom_tgt rel_vers
+    (TVIEWW: sim_tview f flag_src rel_vers tvw_src tvw_tgt)
+    (PROMISES: sim_promises flag_src flag_tgt f vers prom_src prom_tgt)
+    (RELVERS: wf_release_vers vers prom_tgt rel_vers)
+    (FLAGTGT: forall loc ts (FLAG: flag_tgt loc = Some ts),
+        tvw_src.(TView.cur).(View.rlx) loc = ts)
+    (FLAGSRC: forall loc ts (FLAG: flag_src loc = Some ts),
+        tvw_src.(TView.cur).(View.rlx) loc = ts)
+  :
+    sim_local
+      f vers flag_src flag_tgt
+      (Local.mk tvw_src prom_src)
+      (Local.mk tvw_tgt prom_tgt)
+.
+
+Lemma sim_local_tgt_mon f vers flag_src flag_tgt lc_src lc_tgt0 lc_tgt1
+      (SIM: sim_local f vers flag_src flag_tgt lc_src lc_tgt0)
+      (PROM: lc_tgt0.(Local.promises) = lc_tgt1.(Local.promises))
+      (TVIEW: TView.le lc_tgt0.(Local.tview) lc_tgt1.(Local.tview))
+  :
+    sim_local f vers flag_src flag_tgt lc_src lc_tgt1.
+Proof.
+  inv SIM. destruct lc_tgt1. ss. clarify. econs; eauto.
+  eapply sim_tview_tgt_mon; eauto.
+Qed.
+
+Lemma sim_local_consistent f vers flag_src flag_tgt lc_src lc_tgt
+      (CONSISTENT: Local.promise_consistent lc_tgt)
+      (SIM: sim_local f vers flag_src flag_tgt lc_src lc_tgt)
+      (WF: Mapping.wfs f)
+  :
+    Local.promise_consistent lc_src.
+Proof.
+  inv SIM. ii. ss.
+  hexploit sim_promises_get_if; eauto. i. des.
+  { eapply sim_timestamp_lt.
+    { eapply sim_view_rlx.
+      { eapply sim_tview_cur. eauto. }
+      { ss. destruct (flag_src loc) eqn:FLAG; auto.
+        erewrite sim_promises_none in PROMISE; eauto. ss.
+      }
     }
-    { eapply sim_view_mon_tgt.
-      { eapply SIM. }
-      { eapply TVIEW. }
+    { eauto. }
+    { eapply CONSISTENT; eauto. inv MSG0; ss. }
+    { eauto. }
+    { eapply mapping_latest_wf_loc. }
+  }
+  { eapply FLAGTGT in FLAG. subst. auto. }
+Qed.
+
+Variant max_values_src (vs: Loc.t -> option Const.t)
+        (mem: Memory.t)
+  :
+    forall (lc: Local.t), Prop :=
+| max_values_src_intro
+    tvw prom
+    (MAX: forall loc v0 (VAL: vs loc = Some v0),
+        exists released v1,
+          (<<MAX: max_readable
+                    mem
+                    prom
+                    loc
+                    (tvw.(TView.cur).(View.pln) loc)
+                    v1 released>>) /\
+          (<<VAL: Const.le v0 v1>>))
+    (NONMAX: forall loc (VAL: vs loc = None),
+        forall val released,
+          ~ max_readable mem prom loc (tvw.(TView.cur).(View.pln) loc) val released)
+  :
+    max_values_src vs mem (Local.mk tvw prom)
+.
+
+Variant max_values_tgt (vs: Loc.t -> option Const.t)
+        (mem: Memory.t)
+  :
+    forall (lc: Local.t), Prop :=
+| max_values_tgt_intro
+    tvw prom
+    (MAX: forall loc v1 (VAL: vs loc = Some v1),
+        exists released v0,
+          (<<MAX: max_readable
+                    mem
+                    prom
+                    loc
+                    (tvw.(TView.cur).(View.pln) loc)
+                    v0 released>>) /\
+          (<<VAL: Const.le v0 v1>>))
+  :
+    max_values_tgt vs mem (Local.mk tvw prom)
+.
+
+Lemma max_values_tgt_mon vs mem lc0 lc1
+      (MAXTGT: max_values_tgt vs mem lc0)
+      (PROM: lc0.(Local.promises) = lc1.(Local.promises))
+      (TVIEW: TView.le lc0.(Local.tview) lc1.(Local.tview))
+      (LOCAL: Local.wf lc1 mem)
+      (CONSISTENT: Local.promise_consistent lc1)
+  :
+    max_values_tgt vs mem lc1.
+Proof.
+  inv MAXTGT. ss. subst. destruct lc1. econs. i.
+  hexploit MAX; eauto. i. des. ss.
+  hexploit max_readable_view_mon; eauto.
+Qed.
+
+Variant sim_thread
+        (f: Mapping.ts) (vers: versions)
+        (flag_src: Loc.t -> option Time.t)
+        (flag_tgt: Loc.t -> option Time.t)
+        (vs_src: Loc.t -> option Const.t)
+        (vs_tgt: Loc.t -> option Const.t)
+        mem_src mem_tgt lc_src lc_tgt sc_src sc_tgt: Prop :=
+| sim_thread_intro
+    (SC: sim_timemap (fun _ => True) f (Mapping.vers f) sc_src sc_tgt)
+    (MEM: sim_memory flag_src f vers mem_src mem_tgt)
+    (LOCAL: sim_local f vers flag_src flag_tgt lc_src lc_tgt)
+    (MAXSRC: max_values_src vs_src mem_src lc_src)
+    (MAXTGT: max_values_tgt vs_tgt mem_tgt lc_tgt)
+    (PERM: forall loc, option_rel (fun _ _ => True) (vs_src loc) (vs_tgt loc))
+.
+
+Lemma sim_thread_tgt_read_na
+      f vers flag_src flag_tgt vs_src vs_tgt
+      mem_src mem_tgt lc_src lc_tgt0 sc_src sc_tgt
+      loc to_tgt val_tgt vw_tgt lc_tgt1
+      (READ: Local.read_step lc_tgt0 mem_tgt loc to_tgt val_tgt vw_tgt Ordering.na lc_tgt1)
+      (SIM: sim_thread
+              f vers flag_src flag_tgt vs_src vs_tgt
+              mem_src mem_tgt lc_src lc_tgt0 sc_src sc_tgt)
+      (CONSISTNET: Local.promise_consistent lc_tgt1)
+      (LOCAL: Local.wf lc_tgt0 mem_tgt)
+      (MEM: Memory.closed mem_tgt)
+  :
+    (<<SIM: sim_thread
+              f vers flag_src flag_tgt vs_src vs_tgt
+              mem_src mem_tgt lc_src lc_tgt1 sc_src sc_tgt>>) /\
+    (<<VAL: forall val (VALS: vs_tgt loc = Some val), Const.le val_tgt val>>).
+Proof.
+  hexploit Local.read_step_future; eauto.
+  i. des. splits.
+  { inv SIM. econs; eauto.
+    { eapply sim_local_tgt_mon; eauto.
+      { inv READ; ss. }
     }
-    { eapply sim_view_mon_tgt.
-      { eapply SIM. }
-      { eapply TVIEW. }
+    { eapply max_values_tgt_mon; eauto.
+      { inv READ; ss. }
     }
-  Qed.
+  }
+  { i. inv SIM. inv MAXTGT.
+    hexploit MAX; eauto. i. des.
+    hexploit max_readable_read_only; eauto.
+    i. des; auto. etrans; eauto.
+  }
+Qed.
 
-  Variant wf_release_vers (vers: versions) (prom_tgt: Memory.t) (rel_vers: Loc.t -> version): Prop :=
-  | wf_release_vers_intro
-      (PROM: forall loc from to val released
-                    (GET: Memory.get loc to prom_tgt = Some (from, Message.concrete val (Some released))),
-          exists v,
-            (<<VER: vers loc to = Some v>>) /\
-            (<<REL: rel_vers loc = v>>))
-  .
+Lemma sim_thread_tgt_read_na_racy
+      f vers flag_src flag_tgt vs_src vs_tgt
+      mem_src mem_tgt lc_src lc_tgt0 sc_src sc_tgt
+      loc val_tgt ord
+      (READ: Local.racy_read_step lc_tgt0 mem_tgt loc val_tgt ord)
+      (SIM: sim_thread
+              f vers flag_src flag_tgt vs_src vs_tgt
+              mem_src mem_tgt lc_src lc_tgt0 sc_src sc_tgt)
+      (LOCAL: Local.wf lc_tgt0 mem_tgt)
+  :
+    vs_tgt loc = None.
+Proof.
+  destruct (vs_tgt loc) eqn:VAL; auto.
+  inv SIM. inv MAXTGT. hexploit MAX; eauto. i. des.
+  exfalso. eapply max_readable_not_read_race; eauto.
+  Unshelve.
+Qed.
 
-  Variant sim_local
-          (f: Mapping.ts) (vers: versions)
-          (flag_src: Loc.t -> option Time.t)
-          (flag_tgt: Loc.t -> option Time.t)
-    :
-      Local.t -> Local.t -> Prop :=
-  | sim_local_intro
-      tvw_src tvw_tgt prom_src prom_tgt rel_vers
-      (TVIEWW: sim_tview f flag_src rel_vers tvw_src tvw_tgt)
-      (PROMISES: sim_promises flag_src flag_tgt f vers prom_src prom_tgt)
-      (RELVERS: wf_release_vers vers prom_tgt rel_vers)
-      (FLAGTGT: forall loc ts (FLAG: flag_tgt loc = Some ts),
-          tvw_src.(TView.cur).(View.rlx) loc = ts)
-      (FLAGSRC: forall loc ts (FLAG: flag_src loc = Some ts),
-          tvw_src.(TView.cur).(View.rlx) loc = ts)
-    :
-      sim_local
-        f vers flag_src flag_tgt
-        (Local.mk tvw_src prom_src)
-        (Local.mk tvw_tgt prom_tgt)
-  .
+Lemma sim_thread_src_read_na
+      f vers flag_src flag_tgt vs_src vs_tgt
+      mem_src mem_tgt lc_src lc_tgt sc_src sc_tgt
+      loc val_src val
+      (SIM: sim_thread
+              f vers flag_src flag_tgt vs_src vs_tgt
+              mem_src mem_tgt lc_src lc_tgt sc_src sc_tgt)
+      (VALS: vs_src loc = Some val)
+      (VAL: Const.le val_src val)
+      (LOCAL: Local.wf lc_src mem_src)
+  :
+    exists to vw,
+      Local.read_step lc_src mem_src loc to val_src vw Ordering.na lc_src.
+Proof.
+  inv SIM. inv MAXSRC. hexploit MAX; eauto. i. des.
+  hexploit max_readable_read.
+  { eauto. }
+  { eauto. }
+  { eauto. }
+  { instantiate (1:=val_src). etrans; eauto. }
+  i. des. esplits; eauto.
+Qed.
 
-  Lemma sim_local_tgt_mon f vers flag_src flag_tgt lc_src lc_tgt0 lc_tgt1
-        (SIM: sim_local f vers flag_src flag_tgt lc_src lc_tgt0)
-        (PROM: lc_tgt0.(Local.promises) = lc_tgt1.(Local.promises))
-        (TVIEW: TView.le lc_tgt0.(Local.tview) lc_tgt1.(Local.tview))
-    :
-      sim_local f vers flag_src flag_tgt lc_src lc_tgt1.
-  Proof.
-    inv SIM. destruct lc_tgt1. ss. clarify. econs; eauto.
-    eapply sim_tview_tgt_mon; eauto.
-  Qed.
+Lemma sim_thread_src_read_na_racy
+      f vers flag_src flag_tgt vs_src vs_tgt
+      mem_src mem_tgt lc_src lc_tgt sc_src sc_tgt
+      loc val_src
+      (SIM: sim_thread
+              f vers flag_src flag_tgt vs_src vs_tgt
+              mem_src mem_tgt lc_src lc_tgt sc_src sc_tgt)
+      (CONSISTNET: Local.promise_consistent lc_tgt)
+      (LOCAL: Local.wf lc_src mem_src)
+      (VALS: vs_src loc = None)
+      (WF: Mapping.wfs f)
+  :
+    Local.racy_read_step lc_src mem_src loc val_src Ordering.na.
+Proof.
+  inv SIM. inv MAXSRC.
+  hexploit non_max_readable_read; eauto.
+  eapply sim_local_consistent; eauto.
+Qed.
 
-  Lemma sim_local_consistent f vers flag_src flag_tgt lc_src lc_tgt
-        (CONSISTENT: Local.promise_consistent lc_tgt)
-        (SIM: sim_local f vers flag_src flag_tgt lc_src lc_tgt)
-        (WF: Mapping.wfs f)
-    :
-      Local.promise_consistent lc_src.
-  Proof.
-    inv SIM. ii. ss.
-    hexploit sim_promises_get_if; eauto. i. des.
-    { eapply sim_timestamp_lt.
-      { eapply sim_view_rlx.
-        { eapply sim_tview_cur. eauto. }
-        { ss. destruct (flag_src loc) eqn:FLAG; auto.
-          erewrite sim_promises_none in PROMISE; eauto. ss.
+Lemma sim_thread_tgt_write_na_racy
+      f vers flag_src flag_tgt vs_src vs_tgt
+      mem_src mem_tgt lc_src lc_tgt0 sc_src sc_tgt
+      loc
+      (WRITE: Local.racy_write_step lc_tgt0 mem_tgt loc Ordering.na)
+      (SIM: sim_thread
+              f vers flag_src flag_tgt vs_src vs_tgt
+              mem_src mem_tgt lc_src lc_tgt0 sc_src sc_tgt)
+      (LOCAL: Local.wf lc_tgt0 mem_tgt)
+  :
+    vs_tgt loc = None.
+Proof.
+  destruct (vs_tgt loc) eqn:VAL; auto.
+  inv SIM. inv MAXTGT. hexploit MAX; eauto. i. des.
+  exfalso. eapply max_readable_not_write_race; eauto.
+Qed.
+
+Lemma sim_thread_src_write_na_racy
+      f vers flag_src flag_tgt vs_src vs_tgt
+      mem_src mem_tgt lc_src lc_tgt sc_src sc_tgt
+      loc
+      (SIM: sim_thread
+              f vers flag_src flag_tgt vs_src vs_tgt
+              mem_src mem_tgt lc_src lc_tgt sc_src sc_tgt)
+      (CONSISTNET: Local.promise_consistent lc_tgt)
+      (LOCAL: Local.wf lc_src mem_src)
+      (VALS: vs_src loc = None)
+      (WF: Mapping.wfs f)
+  :
+    Local.racy_write_step lc_src mem_src loc Ordering.na.
+Proof.
+  inv SIM. inv MAXSRC.
+  hexploit non_max_readable_write; eauto.
+  eapply sim_local_consistent; eauto.
+Qed.
+
+Lemma cap_max_readable mem cap prom loc ts val released
+      (CAP: Memory.cap mem cap)
+      (MLE: Memory.le prom mem)
+      (MEM: Memory.closed mem)
+  :
+    max_readable mem prom loc ts val released
+    <->
+    max_readable cap prom loc ts val released.
+Proof.
+  split.
+  { i. inv H. econs; eauto.
+    { eapply Memory.cap_le; [..|eauto]; eauto. refl. }
+    { i. eapply Memory.cap_inv in GET0; eauto. des; clarify.
+      eapply MAX in GET0; eauto.
+    }
+  }
+  { i. inv H. eapply Memory.cap_inv in GET; eauto. des; clarify.
+    econs; eauto. i. eapply MAX; eauto.
+    eapply Memory.cap_le; [..|eauto]; eauto. refl.
+  }
+Qed.
+
+Lemma cap_max_values_src vs mem cap lc
+      (MAX: max_values_src vs mem lc)
+      (CAP: Memory.cap mem cap)
+      (LOCAL: Local.wf lc mem)
+      (MEM: Memory.closed mem)
+  :
+    max_values_src vs cap lc.
+Proof.
+  inv MAX. econs.
+  { i. hexploit MAX0; eauto. i. des. esplits; eauto.
+    erewrite <- cap_max_readable; eauto. eapply LOCAL.
+  }
+  { i. hexploit NONMAX; eauto. ii. eapply H.
+    erewrite cap_max_readable; eauto. eapply LOCAL.
+  }
+Qed.
+
+Lemma cap_max_values_tgt vs mem cap lc
+      (MAX: max_values_tgt vs mem lc)
+      (CAP: Memory.cap mem cap)
+      (LOCAL: Local.wf lc mem)
+      (MEM: Memory.closed mem)
+  :
+    max_values_tgt vs cap lc.
+Proof.
+  inv MAX. econs.
+  i. hexploit MAX0; eauto. i. des. esplits; eauto.
+  erewrite <- cap_max_readable; eauto. eapply LOCAL.
+Qed.
+
+Lemma sim_promises_preserve
+      prom_src prom_tgt flag_src flag_tgt f0 f1 vers mem
+      (SIM: sim_promises flag_src flag_tgt f0 vers prom_src prom_tgt)
+      (MAPLE: Mapping.les f0 f1)
+      (PRESERVE: forall loc to from msg
+                        (GET: Memory.get loc to mem = Some (from, msg))
+                        ts fts
+                        (TS: Time.le ts to)
+                        (MAP: sim_timestamp_exact (f0 loc) (f0 loc).(Mapping.ver) fts ts),
+          sim_timestamp_exact (f1 loc) (f1 loc).(Mapping.ver) fts ts)
+      (MLE: Memory.le prom_tgt mem)
+      (WF: Mapping.wfs f0)
+      (VERS: versions_wf f0 vers)
+  :
+    sim_promises flag_src flag_tgt f1 vers prom_src prom_tgt.
+Proof.
+  econs.
+  { i. hexploit sim_promises_get; eauto. i. des. esplits.
+    { eapply PRESERVE; eauto. eapply memory_get_ts_le; eauto. }
+    { eapply PRESERVE; eauto. refl. }
+    { eauto. }
+    { erewrite <- sim_message_max_mon_mapping; eauto. }
+  }
+  { i. hexploit sim_promises_get_if; eauto. i. des.
+    { left. esplits.
+      { eapply PRESERVE; eauto. refl. }
+      { eauto. }
+    }
+    { right. esplits; eauto. }
+  }
+  { i. eapply sim_promises_none; eauto. }
+Qed.
+
+Lemma sim_thread_cap
+      f0 vers flag_tgt vs_src vs_tgt
+      mem_src mem_tgt lc_src lc_tgt sc_src sc_tgt
+      cap_src cap_tgt
+      (SIM: sim_thread
+              f0 vers (fun _ => None) flag_tgt vs_src vs_tgt
+              mem_src mem_tgt lc_src lc_tgt sc_src sc_tgt)
+      (CAPSRC: Memory.cap mem_src cap_src)
+      (CAPTGT: Memory.cap mem_tgt cap_tgt)
+      (WF: Mapping.wfs f0)
+      (VERS: versions_wf f0 vers)
+      (MEMSRC: Memory.closed mem_src)
+      (MEMTGT: Memory.closed mem_tgt)
+      (LOCALSRC: Local.wf lc_src mem_src)
+      (LOCALTGT: Local.wf lc_tgt mem_tgt)
+  :
+    exists f1,
+      (<<MAPLE: Mapping.les f0 f1>>) /\
+      (<<MAPWF: Mapping.wfs f1>>) /\
+      (<<SIM: sim_thread
+                f1 vers (fun _ => None) flag_tgt vs_src vs_tgt
+                cap_src cap_tgt lc_src lc_tgt sc_src sc_tgt>>) /\
+      (<<VERS: versions_wf f1 vers>>)
+.
+Proof.
+  inv SIM. hexploit cap_sim_memory; eauto. i. des. esplits; eauto.
+  2:{ eapply versions_wf_mapping_mon; eauto. }
+  econs; eauto.
+  { eapply sim_timemap_mon_latest; eauto. }
+  { inv LOCAL. econs; eauto.
+    { eapply sim_tview_mon_latest; eauto. }
+    { eapply sim_promises_preserve; eauto. eapply LOCALTGT. }
+  }
+  { eapply cap_max_values_src; eauto. }
+  { eapply cap_max_values_tgt; eauto. }
+Qed.
+
+Lemma local_write_step_write_na_step
+      lc0 sc0 mem0 loc from to val releasedm released lc1 sc1 mem1 kind
+      (WRITE: Local.write_step lc0 sc0 mem0 loc from to val releasedm released Ordering.na lc1 sc1 mem1 kind)
+  :
+    Local.write_na_step lc0 sc0 mem0 loc from to val Ordering.na lc1 sc1 mem1 [] [] kind.
+Proof.
+  inv WRITE. econs; eauto. econs.
+  { eapply WRITABLE. }
+  exact WRITE0.
+Qed.
+
+Lemma sim_readable L f vw_src vw_tgt loc to_src to_tgt released_src released_tgt ord
+      (READABLE: TView.readable vw_tgt loc to_tgt released_tgt ord)
+      (SIM: sim_view L f (Mapping.vers f) vw_src vw_tgt)
+      (TO: sim_timestamp_exact (f loc) (f loc).(Mapping.ver) to_src to_tgt)
+      (WF: Mapping.wfs f)
+      (LOC: L loc)
+  :
+    TView.readable vw_src loc to_src released_src ord.
+Proof.
+  inv READABLE. econs.
+  { eapply sim_timestamp_le.
+    { eapply SIM. auto. }
+    { eauto. }
+    { eauto. }
+    { eauto. }
+    { eapply mapping_latest_wf_loc. }
+  }
+  { i. eapply sim_timestamp_le.
+    { eapply SIM. auto. }
+    { eauto. }
+    { eauto. }
+    { eauto. }
+    { eapply mapping_latest_wf_loc. }
+  }
+Qed.
+
+Lemma sim_writable L f vw_src vw_tgt loc to_src to_tgt sc_src sc_tgt ord
+      (WRITABLE: TView.writable vw_tgt sc_tgt loc to_tgt ord)
+      (SIM: sim_view L f (Mapping.vers f) vw_src vw_tgt)
+      (TO: sim_timestamp_exact (f loc) (f loc).(Mapping.ver) to_src to_tgt)
+      (WF: Mapping.wfs f)
+      (LOC: L loc)
+  :
+    TView.writable vw_src sc_src loc to_src ord.
+Proof.
+  inv WRITABLE. econs.
+  eapply sim_timestamp_lt.
+  { eapply SIM. auto. }
+  { eauto. }
+  { eauto. }
+  { eauto. }
+  { eapply mapping_latest_wf_loc. }
+Qed.
+
+Lemma sim_view_singleton_ur_if l (L: Loc.t -> Prop) f v
+      ts_src ts_tgt cond
+      (SIM: L l -> sim_timestamp (f l) (v l) ts_src ts_tgt)
+      (WF: Mapping.wfs f)
+      (VERWF: version_wf f v)
+  :
+    sim_view L f v (View.singleton_ur_if cond l ts_src) (View.singleton_ur_if cond l ts_tgt).
+Proof.
+  unfold View.singleton_ur_if. des_ifs.
+  { eapply sim_view_singleton_ur; eauto. }
+  { eapply sim_view_singleton_rw; eauto. }
+Qed.
+
+Lemma message_to_time_le_opt_view loc to val released
+      (MSGTO: Memory.message_to (Message.concrete val released) loc to)
+  :
+    time_le_opt_view loc to released.
+Proof.
+  invMS
+
+      loc to
+
+
+time_le_opt_view
+
+Lemma sim_read_tview f flag_src flag_tgt tvw_src tvw_tgt
+      loc to_src released_src ord to_tgt released_tgt
+      (SIM: sim_tview f flag_src flag_tgt tvw_src tvw_tgt)
+      (TO: sim_timestamp_exact (f loc) (f loc).(Mapping.ver) to_src to_tgt)
+      (CLOSED: Mapping.closed (f loc) (Mapping.vers f loc) to_src)
+      (WF: Mapping.wfs f)
+  :
+    sim_tview f flag_src flag_tgt (TView.read_tview tvw_src loc to_src released_src ord) (TView.read_tview tvw_tgt loc to_tgt released_tgt ord).
+Proof.
+  pose proof (mapping_latest_wf f).
+  econs.
+  { eapply SIM. }
+  { ss. rewrite View.join_assoc. rewrite View.join_assoc.
+    eapply sim_view_join; eauto.
+    { eapply SIM. }
+    unfold View.singleton_ur_if. des_ifs.
+    { admit. }
+    { admit. }
+    { destruct ord; ss. }
+    { admit. }
+  }
+
+    {
+
+
+eapply sim_view_join; eauto.
+      { eapply SIM. }
+      { eapply sim_view_singleton_ur_if; eauto.
+        i. eapply sim_timestamp_exact_sim; eauto.
+      }
+    }
+    { des_ifs.
+      { admit. }
+      { eapply sim_view_join; eauto.
+        { eapply sim_view_join; eauto.
+          { eapply SIM. }
+          { ss. eapply sim_view_singleton_rw; eauto.
+            i. eapply sim_timestamp_exact_sim; eauto.
+          }
         }
+        { eapply sim_view_bot; eauto. }
       }
-      { eauto. }
-      { eapply CONSISTENT; eauto. inv MSG0; ss. }
-      { eauto. }
-      { eapply mapping_latest_wf_loc. }
     }
-    { eapply FLAGTGT in FLAG. subst. auto. }
-  Qed.
+    { eapply SIM. }
+Admitted.
 
-  Variant max_values_src (vs: Loc.t -> option Const.t)
-          (mem: Memory.t)
-    :
-      forall (lc: Local.t), Prop :=
-  | max_values_src_intro
-      tvw prom
-      (MAX: forall loc v (VAL: vs loc = Some v),
-          exists released,
-            (<<MAX: max_readable
-                      mem
-                      prom
-                      loc
-                      (tvw.(TView.cur).(View.pln) loc)
-                      v released>>))
-      (NONMAX: forall loc (VAL: vs loc = None),
-          forall val released,
-            ~ max_readable mem prom loc (tvw.(TView.cur).(View.pln) loc) val released)
-    :
-      max_values_src vs mem (Local.mk tvw prom)
-  .
-
-  Variant max_values_tgt (vs: Loc.t -> option Const.t)
-          (mem: Memory.t)
-    :
-      forall (lc: Local.t), Prop :=
-  | max_values_tgt_intro
-      tvw prom
-      (MAX: forall loc v (VAL: vs loc = Some v),
-          exists released,
-            (<<MAX: max_readable
-                      mem
-                      prom
-                      loc
-                      (tvw.(TView.cur).(View.pln) loc)
-                      v released>>))
-    :
-      max_values_tgt vs mem (Local.mk tvw prom)
-  .
-
-  Lemma max_values_tgt_mon vs mem lc0 lc1
-        (MAXTGT: max_values_tgt vs mem lc0)
-        (PROM: lc0.(Local.promises) = lc1.(Local.promises))
-        (TVIEW: TView.le lc0.(Local.tview) lc1.(Local.tview))
-        (LOCAL: Local.wf lc1 mem)
-        (CONSISTENT: Local.promise_consistent lc1)
-    :
-      max_values_tgt vs mem lc1.
-  Proof.
-    inv MAXTGT. ss. subst. destruct lc1. econs. i.
-    hexploit MAX; eauto. i. des. ss.
-    hexploit max_readable_view_mon; eauto.
-  Qed.
-
-  Variant sim_thread
-          (f: Mapping.ts) (vers: versions)
-          (flag_src: Loc.t -> option Time.t)
-          (flag_tgt: Loc.t -> option Time.t)
-          (vs_src: Loc.t -> option Const.t)
-          (vs_tgt: Loc.t -> option Const.t)
-          mem_src mem_tgt lc_src lc_tgt sc_src sc_tgt: Prop :=
-  | sim_thread_intro
-      (SC: sim_timemap (fun _ => True) f (Mapping.vers f) sc_src sc_tgt)
-      (MEM: sim_memory flag_src f vers mem_src mem_tgt)
-      (LOCAL: sim_local f vers flag_src flag_tgt lc_src lc_tgt)
-      (MAXSRC: max_values_src vs_src mem_src lc_src)
-      (MAXTGT: max_values_tgt vs_tgt mem_tgt lc_tgt)
-      (PERM: forall loc, option_rel (fun _ _ => True) (vs_src loc) (vs_tgt loc))
-      (VERS: versions_wf f vers)
-  .
-
-  Lemma sim_thread_tgt_read_na
-        f vers flag_src flag_tgt vs_src vs_tgt
-        mem_src mem_tgt lc_src lc_tgt0 sc_src sc_tgt
-        loc to_tgt val_tgt vw_tgt lc_tgt1
-        (READ: Local.read_step lc_tgt0 mem_tgt loc to_tgt val_tgt vw_tgt Ordering.na lc_tgt1)
-        (SIM: sim_thread
-                f vers flag_src flag_tgt vs_src vs_tgt
-                mem_src mem_tgt lc_src lc_tgt0 sc_src sc_tgt)
-        (CONSISTNET: Local.promise_consistent lc_tgt1)
-        (LOCAL: Local.wf lc_tgt0 mem_tgt)
-        (MEM: Memory.closed mem_tgt)
-    :
+Lemma sim_thread_read
+      f vers flag_src flag_tgt vs_src0 vs_tgt0
+      mem_src mem_tgt lc_src0 lc_tgt0 sc_src sc_tgt
+      loc to_tgt val released_tgt ord lc_tgt1
+      (READ: Local.read_step lc_tgt0 mem_tgt loc to_tgt val released_tgt ord lc_tgt1)
+      (SIM: sim_thread
+              f vers flag_src flag_tgt vs_src0 vs_tgt0
+              mem_src mem_tgt lc_src0 lc_tgt0 sc_src sc_tgt)
+      (CONSISTNET: Local.promise_consistent lc_tgt1)
+      (LOCAL: Local.wf lc_tgt0 mem_tgt)
+      (MEM: Memory.closed mem_tgt)
+      (FLAGSRC: flag_src loc = None)
+      (FLAGTGT: flag_tgt loc = None)
+      (ACQ: forall loc (ORD: Ordering.le Ordering.acqrel ord)
+                   (FLAG: flag_src loc = None),
+          flag_tgt loc = None)
+      (WF: Mapping.wfs f)
+  :
+    exists lc_src1 to_src released_src vs_src1 vs_tgt1,
+      (<<READ: Local.read_step lc_src0 mem_src loc to_src val released_src ord lc_src1>>) /\
+      (<<TO: sim_timestamp_exact (f loc) (f loc).(Mapping.ver) to_src to_tgt>>) /\
+      (<<RELEASED: sim_opt_view (fun loc0 => loc0 <> loc) f (vers loc to_tgt) released_src released_tgt>>) /\
       (<<SIM: sim_thread
-                f vers flag_src flag_tgt vs_src vs_tgt
-                mem_src mem_tgt lc_src lc_tgt1 sc_src sc_tgt>>) /\
-      (<<VAL: forall val (VAL: vs_tgt loc = Some val), Const.le val_tgt val>>).
-  Proof.
-    hexploit Local.read_step_future; eauto.
-    i. des. splits.
-    { inv SIM. econs; eauto.
-      { eapply sim_local_tgt_mon; eauto.
-        { inv READ; ss. }
-      }
-      { eapply max_values_tgt_mon; eauto.
-        { inv READ; ss. }
-      }
+                f vers flag_src flag_tgt vs_src1 vs_tgt1
+                mem_src mem_tgt lc_src0 lc_tgt1 sc_src sc_tgt>>)
+.
+Proof.
+  inv READ. inv SIM.
+  hexploit sim_memory_get; eauto; ss. i. des.
+  inv MSG; ss. esplits.
+  { econs; ss.
+    { eauto. }
+    { etrans; eauto. }
+    { inv LOCAL0. eapply sim_readable; eauto.
+      { eapply sim_tview_cur. eauto. }
+      { ss. }
     }
-    { i. inv SIM. inv MAXTGT.
-      hexploit MAX; eauto. i. des.
-      hexploit max_readable_read_only; eauto.
-      i. des. auto.
-    }
-  Qed.
+  }
+  { eauto. }
+  { rewrite H0. admit. }
+  { econs; eauto.
+    { inv LOCAL0. econs; eauto. ss. admit. }
+    { admit. }
+  }
+Admitted.
 
-  Lemma sim_thread_tgt_read_na_racy
-        f vers flag_src flag_tgt vs_src vs_tgt
-        mem_src mem_tgt lc_src lc_tgt0 sc_src sc_tgt
-        loc val_tgt ord
-        (READ: Local.racy_read_step lc_tgt0 mem_tgt loc val_tgt ord)
-        (SIM: sim_thread
-                f vers flag_src flag_tgt vs_src vs_tgt
-                mem_src mem_tgt lc_src lc_tgt0 sc_src sc_tgt)
-        (LOCAL: Local.wf lc_tgt0 mem_tgt)
-    :
-      vs_tgt loc = None.
-  Proof.
-    destruct (vs_tgt loc) eqn:VAL; auto.
-    inv SIM. inv MAXTGT. hexploit MAX; eauto. i. des.
-    exfalso. eapply max_readable_not_read_race; eauto.
-  Qed.
+Lemma sim_thread_tgt_write_na
+      f vers flag_src flag_tgt vs_src vs_tgt
+      mem_src mem_tgt0 lc_src lc_tgt0 sc_src sc_tgt0
+      loc from_tgt to_tgt val_tgt lc_tgt1 sc_tgt1 mem_tgt1 msgs kinds kind
+      (WRITE: Local.write_na_step lc_tgt0 sc_tgt0 mem_tgt0 loc from_tgt to_tgt val_tgt Ordering.na lc_tgt1 sc_tgt1 mem_tgt1 msgs kinds kind)
+      (SIM: sim_thread
+              f vers flag_src flag_tgt vs_src vs_tgt
+              mem_src mem_tgt0 lc_src lc_tgt0 sc_src sc_tgt0)
+      (CONSISTNET: Local.promise_consistent lc_tgt1)
+      (LOCAL: Local.wf lc_tgt0 mem_tgt0)
+      (MEM: Memory.closed mem_tgt0)
+      (VAL: vs_tgt loc <> None)
+      (LOWER: mem_tgt1 = mem_tgt0)
+  :
+    sim_thread
+      f vers flag_src flag_tgt vs_src
+      (fun loc0 => if Loc.eq_dec loc0 loc then (Some val_tgt) else (vs_tgt loc0))
+      mem_src mem_tgt1 lc_src lc_tgt1 sc_src sc_tgt1.
+Proof.
+  inv SIM. econs; eauto.
+  { inv WRITE. eauto. }
+  { inv WRITE. econs; eauto. ss. inv LOCAL. econs.
 
-  Lemma sim_thread_tgt_read_na
-        f vers flag_src flag_tgt vs_src vs_tgt
-        mem_src mem_tgt lc_src lc_tgt0 sc_src sc_tgt
-        loc to_tgt val_tgt vw_tgt lc_tgt1
-        (READ: Local.read_step lc_tgt0 mem_tgt loc to_tgt val_tgt vw_tgt Ordering.na lc_tgt1)
-        (SIM: sim_thread
-                f vers flag_src flag_tgt vs_src vs_tgt
-                mem_src mem_tgt lc_src lc_tgt0 sc_src sc_tgt)
-        (CONSISTNET: Local.promise_consistent lc_tgt1)
-        (LOCAL: Local.wf lc_tgt0 mem_tgt)
-        (MEM: Memory.closed mem_tgt)
-    :
-      (<<SIM: sim_thread
-                f vers flag_src flag_tgt vs_src vs_tgt
-                mem_src mem_tgt lc_src lc_tgt1 sc_src sc_tgt>>) /\
-      (<<VAL: forall val (VAL: vs_tgt loc = Some val), Const.le val_tgt val>>).
-  Proof.
-    hexploit Local.read_step_future; eauto.
-    i. des. splits.
-    { inv SIM. econs; eauto.
-      { eapply sim_local_tgt_mon; eauto.
-        { inv READ; ss. }
-      }
-      { eapply max_values_tgt_mon; eauto.
-        { inv READ; ss. }
-      }
-    }
-    { i. inv SIM. inv MAXTGT.
-      hexploit MAX; eauto. i. des.
-      hexploit max_readable_read_only; eauto.
-      i. des. auto.
-    }
-  Qed.
+admit. }
+  { admit. }
+  { i. specialize (PERM loc0). unfold option_rel in *. des_ifs. }
+Qed.
 
+    inv PERM.
+
+  econs.
+
+
+
+  hexploit Local.read_step_future; eauto.
+  i. des. splits.
+  { inv SIM. econs; eauto.
+    { eapply sim_local_tgt_mon; eauto.
+      { inv READ; ss. }
+    }
+    { eapply max_values_tgt_mon; eauto.
+      { inv READ; ss. }
+    }
+  }
+  { i. inv SIM. inv MAXTGT.
+    hexploit MAX; eauto. i. des.
+    hexploit max_readable_read_only; eauto.
+    i. des. auto.
+  }
+Qed.
+
+
+
+
+  | future
   | promise
-  | cap
-  | promise_to_max
+  | cap (done)
+  | promise_to_max_match
+  | promise_to_max_unmatch
 
-  | na_read_src
+  | na_read_src (done)
   | na_read_tgt (done)
-  | na_racy_read_src
+  | na_racy_read_src (done)
   | na_racy_read_tgt (done)
   | na_write_src
   | na_write_tgt
-  | na_write_read_src
-  | na_write_read_tgt
+  | na_racy_write_src (done)
+  | na_racy_write_tgt (done)
 
-  | step_silent
+  | step_silent (done)
   | step_read
   | step_write
   | step_update
   | step_fence
   | step_syscall
-  | step_write_na
-  | step_racy_read
 
-  | step_failure
-  | step_racy_write
-  | step_racy_update
+  | step_failure (done)
+
+
 
 
   Lemma sim_thread_cap
